Cleaned up Unbalanced and RedBlack set examples

examples/miniML/hol2miniml/okasaki-examples/RedBlackSetScript.sml
@@ -1,45 +1,70 @@
-open bossLib Theory Parse boolTheory pairTheory Defn Tactic boolLib
-open relationTheory miscTheory pred_setTheory pred_setSimps lcsymtacs;
+open preamble;
+open miscTheory pred_setTheory pred_setSimps;
 open ml_translatorLib
 
-val fs = full_simp_tac (srw_ss ())
-val rw = srw_tac []
-val wf_rel_tac = WF_REL_TAC
-val induct_on = Induct_on
-val cases_on = Cases_on;
-val every_case_tac = BasicProvers.EVERY_CASE_TAC;
-val full_case_tac = BasicProvers.FULL_CASE_TAC;
-
 val _ = new_theory "RedBlackSet"
+
+(* Okasaki page 28 *)
 
 val _ = Hol_datatype `
 color = Red | Black`;
 
 val _ = Hol_datatype `
-tree = Empty | Node of color => tree => 'a => tree`;
+tree = Empty | Tree of color => tree => 'a => tree`;
 
 val tree_distinct = fetch "-" "tree_distinct"
 val tree_nchotomy = fetch "-" "tree_nchotomy"
 
-val redblack_set_to_set_def = Define `
-(redblack_set_to_set Empty = {}) ∧
-(redblack_set_to_set (Node _ t1 x t2)  =
-  {x} ∪ redblack_set_to_set t1 ∪ redblack_set_to_set t2)`;
+val tree_to_set_def = Define `
+(tree_to_set Empty = {}) ∧
+(tree_to_set (Tree _ t1 x t2)  = {x} ∪ tree_to_set t1 ∪ tree_to_set t2)`;
 
-val redblack_set_ok_def = Define `
-(redblack_set_ok lt Empty = T) ∧
-(redblack_set_ok lt (Node _ t1 x t2) =
-  redblack_set_ok lt t1 ∧
-  redblack_set_ok lt t2 ∧
-  (!y. y ∈ redblack_set_to_set t1 ⇒ lt y x) ∧
-  (!y. y ∈ redblack_set_to_set t2 ⇒ lt x y))`;
+(* The tree is a binary search tree *)
+val is_bst_def = Define `
+(is_bst lt Empty = T) ∧
+(is_bst lt (Tree _ t1 x t2) =
+  is_bst lt t1 ∧
+  is_bst lt t2 ∧
+  (!y. y ∈ tree_to_set t1 ⇒ lt y x) ∧
+  (!y. y ∈ tree_to_set t2 ⇒ lt x y))`;
 
-val empty_def = Define `
+val not_red_def = Define `
+(not_red (Tree Red t1 x t2) = F) ∧
+(not_red _ = T)`;
+
+val red_black_invariant1_def = Define `
+(red_black_invariant1 Empty = T) ∧ 
+(red_black_invariant1 (Tree Black t1 x t2) =
+  red_black_invariant1 t1 ∧ red_black_invariant1 t2) ∧
+(red_black_invariant1 (Tree Red t1 x t2) =
+  red_black_invariant1 t1 ∧ red_black_invariant1 t2 ∧
+  not_red t1 ∧ not_red t2)`;
+
+(* Count the number of black nodes along every path to the root.  Return NONE
+ * if this number isn't the same along every path *)
+val red_black_invariant2_def = Define `
+(red_black_invariant2 Empty = SOME 0) ∧
+(red_black_invariant2 (Tree c t1 x t2) =
+  case red_black_invariant2 t1 of
+     | NONE => NONE
+     | SOME n =>
+         case red_black_invariant2 t1 of
+            | NONE => NONE
+            | SOME n' =>
+                if n = n' then
+                  if c = Black then
+                    SOME (n + 1)
+                  else
+                    SOME n
+                else
+                  NONE)`;
+
+val empty_def = mlDefine `
 empty = Empty`;
 
-val member_def = Define `
+val member_def = mlDefine `
 (member lt x Empty = F) ∧
-(member lt x (Node _ a y b) =
+(member lt x (Tree _ a y b) =
   if lt x y then
     member lt x a
   else if lt y x then
@@ -47,99 +72,124 @@ val member_def = Define `
   else
     T)`;
 
-val member_thm = Q.store_thm ("member_thm",
-`!lt t x.
-  StrongLinearOrder lt ∧
-  redblack_set_ok lt t
-  ⇒
-  (member lt x t = x ∈ redblack_set_to_set t)`,
-induct_on `t` >>
-rw [member_def, redblack_set_ok_def, redblack_set_to_set_def] >>
-fs [StrongLinearOrder, StrongOrder, irreflexive_def, transitive_def,
-    trichotomous] >>
-metis_tac []);
-
-
 val balance_def = Define `
-(balance Black (Node Red (Node Red a x b) y c) z d =
-  Node Red (Node Black a x b) y (Node Black c z d)) ∧
+(balance Black (Tree Red (Tree Red a x b) y c) z d =
+  Tree Red (Tree Black a x b) y (Tree Black c z d)) ∧
 
-(balance Black (Node Red a x (Node Red b y c)) z d =
-  Node Red (Node Black a x b) y (Node Black c z d)) ∧
+(balance Black (Tree Red a x (Tree Red b y c)) z d =
+  Tree Red (Tree Black a x b) y (Tree Black c z d)) ∧
 
-(balance Black a x (Node Red (Node Red b y c) z d) =
-  Node Red (Node Black a x b) y (Node Black c z d)) ∧
+(balance Black a x (Tree Red (Tree Red b y c) z d) =
+  Tree Red (Tree Black a x b) y (Tree Black c z d)) ∧
 
-(balance Black a x (Node Red b y (Node Red c z d)) =
-  Node Red (Node Black a x b) y (Node Black c z d)) ∧
+(balance Black a x (Tree Red b y (Tree Red c z d)) =
+  Tree Red (Tree Black a x b) y (Tree Black c z d)) ∧
 
-(balance col a x b = Node col a x b)`;
+(balance col a x b = Tree col a x b)`;
 
 val balance_ind = fetch "-" "balance_ind"
 
-(*
-val balance_left_def = Define `
-(balance_left Black (Node Red (Node Red a x b) y c) z d =
-  SOME (Node Red (Node Black a x b) y (Node Black c z d))) ∧
+(* HOL expands the above balance into over 100 cases, so this alternate
+ * definition works better for the translator. *) 
+val balance_left_left_def = mlDefine `
+(balance_left_left (Tree Red (Tree Red a x b) y c) z d =
+  SOME (Tree Red (Tree Black a x b) y (Tree Black c z d))) ∧
+(balance_left_left a x b = NONE)`;
 
-(balance_left Black (Node Red a x (Node Red b y c)) z d =
-  SOME (Node Red (Node Black a x b) y (Node Black c z d))) ∧
+val balance_left_right_def = mlDefine `
+(balance_left_right (Tree Red a x (Tree Red b y c)) z d =
+  SOME (Tree Red (Tree Black a x b) y (Tree Black c z d))) ∧
+(balance_left_right a x b = NONE)`;
 
-(balance_left col a x b = NONE)`;
+val balance_right_left_def = mlDefine `
+(balance_right_left a x (Tree Red (Tree Red b y c) z d) =
+  SOME (Tree Red (Tree Black a x b) y (Tree Black c z d))) ∧
+(balance_right_left a x b = NONE)`;
 
-val balance_right_def = Define `
-(balance_right Black a x (Node Red (Node Red b y c) z d) =
-  SOME (Node Red (Node Black a x b) y (Node Black c z d))) ∧
+val balance_right_right_def = mlDefine `
+(balance_right_right a x (Tree Red b y (Tree Red c z d)) =
+  SOME (Tree Red (Tree Black a x b) y (Tree Black c z d))) ∧
+(balance_right_right a x b = NONE)`;
 
-(balance_right Black a x (Node Red b y (Node Red c z d)) =
-  SOME (Node Red (Node Black a x b) y (Node Black c z d))) ∧
+val balance'_def = mlDefine `
+balance' c a x b =
+  if c = Black then
+    case balance_left_left a x b of
+       | SOME t => t
+       | NONE =>
+           case balance_left_right a x b of
+              | SOME t => t
+              | NONE =>
+                  case balance_right_left a x b of
+                     | SOME t => t
+                     | NONE =>
+                         case balance_right_right a x b of
+                            | SOME t => t
+                            | NONE => Tree c a x b
+  else
+    Tree c a x b`;
 
-(balance_right col a x b = NONE)`;
-*)
+val ins_def = mlDefine `
+(ins lt x Empty = Tree Red Empty x Empty) ∧
+(ins lt x (Tree col a y b) =
+  if lt x y then
+    balance' col (ins lt x a) y b
+  else if lt y x then
+    balance' col a y (ins lt x b)
+  else
+    Tree col a y b)`;
 
-val balance_node = Q.prove (
-`!c t1 x t2. ∃c' t1' x' t2'. (balance c t1 x t2 = Node c' t1' x' t2')`,
+val insert_def = mlDefine `
+insert lt x s =
+  case ins lt x s of
+     | Tree _ a y b => Tree Black a y b`;
+
+
+(* Proof of functional correctness *)
+
+val balance'_correct = Q.prove (
+`!c a x b. balance' c a x b = balance c a x b`,
 recInduct balance_ind >>
-srw_tac [PRED_SET_AC_ss] [balance_def]);
+rw [balance'_def, balance_def, balance_left_left_def, balance_left_right_def,
+    balance_right_left_def, balance_right_right_def]);
 
-val balance_set = Q.prove (
+val balance'_tree = Q.prove (
+`!c t1 x t2. ∃c' t1' x' t2'. (balance' c t1 x t2 = Tree c' t1' x' t2')`,
+recInduct balance_ind >>
+rw [balance'_def, balance_left_left_def, balance_left_right_def,
+    balance_right_left_def, balance_right_right_def]);
+
+val balance'_set = Q.prove (
+`!c t1 x t2. tree_to_set (balance' c t1 x t2) = tree_to_set (Tree c t1 x t2)`,
+recInduct balance_ind >>
+srw_tac [PRED_SET_AC_ss] 
+        [balance'_def, balance_left_left_def, balance_left_right_def,
+         balance_right_left_def, balance_right_right_def, tree_to_set_def]);
+
+val balance'_bst = Q.prove (
 `!c t1 x t2.
-  redblack_set_to_set (balance c t1 x t2) =
-  redblack_set_to_set (Node c t1 x t2)`,
+  transitive lt ∧ is_bst lt (Tree c t1 x t2) 
+  ⇒
+  is_bst lt (balance' c t1 x t2)`,
 recInduct balance_ind >>
-srw_tac [PRED_SET_AC_ss] [balance_def, redblack_set_to_set_def]);
-
-val balance_ok = Q.prove (
-`!c t1 x t2.
-  transitive lt ∧
-  redblack_set_ok lt (Node c t1 x t2) ⇒
-  redblack_set_ok lt (balance c t1 x t2)`,
-recInduct balance_ind >>
-rw [transitive_def, balance_def, redblack_set_ok_def, redblack_set_to_set_def] >>
+rw [transitive_def, balance'_def,  balance_left_left_def,
+    balance_left_right_def, balance_right_left_def, balance_right_right_def,
+    is_bst_def, tree_to_set_def] >>
 metis_tac []);
 
-val ins_def = Define `
-(ins lt x Empty = Node Red Empty x Empty) ∧
-(ins lt x (Node col a y b) =
-  if lt x y then
-    balance col (ins lt x a) y b
-  else if lt y x then
-    balance col a y (ins lt x b)
-  else
-    Node col a y b)`;
-
-val ins_node = Q.prove (
-`!lt x t. ?c t1 y t2. (ins lt x t = Node c t1 y t2)`,
+val ins_tree = Q.prove (
+`!lt x t. ?c t1 y t2. (ins lt x t = Tree c t1 y t2)`,
 cases_on `t` >>
 rw [ins_def] >>
-metis_tac [balance_node]);
+metis_tac [balance'_tree]);
 
 val ins_set = Q.prove (
 `∀lt x t.
-  StrongLinearOrder lt ⇒
-  (redblack_set_to_set (ins lt x t) = {x} ∪ redblack_set_to_set t)`,
+  StrongLinearOrder lt 
+  ⇒
+  (tree_to_set (ins lt x t) = {x} ∪ tree_to_set t)`,
 induct_on `t` >>
-rw [redblack_set_to_set_def, ins_def, balance_set] >>
+rw [tree_to_set_def, ins_def, balance'_set] >>
 fs [] >>
 srw_tac [PRED_SET_AC_ss] [] >>
 `x = a` by (fs [StrongLinearOrder, StrongOrder, irreflexive_def,
@@ -147,76 +197,52 @@ srw_tac [PRED_SET_AC_ss] [] >>
             metis_tac []) >>
 rw []);
 
-val ins_ok = Q.prove (
-`!lt x t.
-  StrongLinearOrder lt ∧
-  redblack_set_ok lt t
-  ⇒
-  redblack_set_ok lt (ins lt x t)`,
+val ins_bst = Q.prove (
+`!lt x t. StrongLinearOrder lt ∧ is_bst lt t ⇒ is_bst lt (ins lt x t)`,
 induct_on `t` >>
-rw [redblack_set_ok_def, ins_def, redblack_set_to_set_def] >>
-match_mp_tac balance_ok >>
-rw [redblack_set_ok_def] >>
+rw [is_bst_def, ins_def, tree_to_set_def] >>
+match_mp_tac balance'_bst >>
+rw [is_bst_def] >>
 imp_res_tac ins_set >>
 fs [StrongLinearOrder, StrongOrder]);
 
-val insert_def = Define `
-insert lt x s =
-  case ins lt x s of
-     | Node _ a y b => Node Black a y b`;
-
 val insert_set = Q.store_thm ("insert_set",
 `∀lt x t.
-  StrongLinearOrder lt ⇒
-  (redblack_set_to_set (insert lt x t) = {x} ∪ redblack_set_to_set t)`,
+  StrongLinearOrder lt 
+  ⇒
+  (tree_to_set (insert lt x t) = {x} ∪ tree_to_set t)`,
 rw [insert_def] >>
-`?c t1 y t2. ins lt x t = Node c t1 y t2` by metis_tac [ins_node] >>
-rw [redblack_set_to_set_def] >>
-`redblack_set_to_set (ins lt x t) = redblack_set_to_set (Node c t1 y t2)`
+`?c t1 y t2. ins lt x t = Tree c t1 y t2` by metis_tac [ins_tree] >>
+rw [tree_to_set_def] >>
+`tree_to_set (ins lt x t) = tree_to_set (Tree c t1 y t2)`
          by metis_tac [] >>
 fs [] >>
 imp_res_tac ins_set >>
-fs [redblack_set_to_set_def]);
+fs [tree_to_set_def]);
 
-val insert_ok = Q.store_thm ("insert_ok",
+val insert_ok = Q.store_thm ("insert_bst",
 `!lt x t.
-  StrongLinearOrder lt ∧
-  redblack_set_ok lt t
+  StrongLinearOrder lt ∧ is_bst lt t
   ⇒
-  redblack_set_ok lt (insert lt x t)`,
+  is_bst lt (insert lt x t)`,
 rw [insert_def] >>
-`?c t1 y t2. ins lt x t = Node c t1 y t2` by metis_tac [ins_node] >>
+`?c t1 y t2. ins lt x t = Tree c t1 y t2` by metis_tac [ins_tree] >>
 rw [] >>
-`redblack_set_ok lt (Node c t1 y t2)` by metis_tac [ins_ok] >>
-fs [redblack_set_ok_def]);
+`is_bst lt (Tree c t1 y t2)` by metis_tac [ins_bst] >>
+fs [is_bst_def]);
 
+val member_correct = Q.store_thm ("member_correct",
+`!lt t x.
+  StrongLinearOrder lt ∧
+  is_bst lt t
+  ⇒
+  (member lt x t = x ∈ tree_to_set t)`,
+induct_on `t` >>
+rw [member_def, is_bst_def, tree_to_set_def] >>
+fs [StrongLinearOrder, StrongOrder, irreflexive_def, transitive_def,
+    trichotomous] >>
+metis_tac []);
 
-(* translating balance *)
-
-val balance_def = Define `
-  balance col a x b =
-    if col = Black then
-      case (a,x,b) of
-      | ((Node Red (Node Red a x b) y c),z,d) =>
-        Node Red (Node Black a x b) y (Node Black c z d)
-      | ((Node Red a x (Node Red b y c)),z,d) =>
-        Node Red (Node Black a x b) y (Node Black c z d)
-      | (a,x,(Node Red (Node Red b y c) z d)) =>
-        Node Red (Node Black a x b) y (Node Black c z d)
-      | (a,x,(Node Red b y (Node Red c z d))) =>
-        Node Red (Node Black a x b) y (Node Black c z d)
-      | _ =>
-        Node col a x b
-    else Node col a x b`
-
-val _ = translate balance_def;
-
-(*
-
-val _ = translate member_def;
-val _ = translate ins_def;
-val _ = translate insert_def;
-
-*)
+(* TODO: verify that insert perserves the red-black invariants *)
 
 val _ = export_theory ();
