examples/miniML/hol2miniml/okasaki-examples/UnbalancedSetScript.sml
@@ -1,39 +1,33 @@
-open bossLib Theory Parse boolTheory pairTheory Defn Tactic boolLib
-open relationTheory miscTheory pred_setTheory pred_setSimps lcsymtacs;
+open preamble
+open miscTheory pred_setTheory pred_setSimps 
 open ml_translatorLib;
-
-val fs = full_simp_tac (srw_ss ())
-val rw = srw_tac []
-val wf_rel_tac = WF_REL_TAC
-val induct_on = Induct_on
-val cases_on = Cases_on;
-val every_case_tac = BasicProvers.EVERY_CASE_TAC;
-val full_case_tac = BasicProvers.FULL_CASE_TAC;
 
 val _ = new_theory "UnbalancedSet"
 
+(* Okasaki page 14 *)
+
 val _ = Hol_datatype `
-tree = Empty | Node of tree => 'a => tree`;
+tree = Empty | Tree of tree => 'a => tree`;
 
-val unbalanced_set_to_set_def = Define `
-(unbalanced_set_to_set Empty = {}) ∧
-(unbalanced_set_to_set (Node t1 x t2)  =
-  {x} ∪ unbalanced_set_to_set t1 ∪ unbalanced_set_to_set t2)`;
+val tree_to_set_def = Define `
+(tree_to_set Empty = {}) ∧
+(tree_to_set (Tree t1 x t2) = {x} ∪ tree_to_set t1 ∪ tree_to_set t2)`;
 
-val unbalanced_set_ok_def = Define `
-(unbalanced_set_ok lt Empty = T) ∧
-(unbalanced_set_ok lt (Node t1 x t2) =
-  unbalanced_set_ok lt t1 ∧
-  unbalanced_set_ok lt t2 ∧
-  (!y. y ∈ unbalanced_set_to_set t1 ⇒ lt y x) ∧
-  (!y. y ∈ unbalanced_set_to_set t2 ⇒ lt x y))`;
+(* That the tree is a binary search tree *)
+val is_bst_def = Define `
+(is_bst lt Empty = T) ∧
+(is_bst lt (Tree t1 x t2) =
+  is_bst lt t1 ∧
+  is_bst lt t2 ∧
+  (!y. y ∈ tree_to_set t1 ⇒ lt y x) ∧
+  (!y. y ∈ tree_to_set t2 ⇒ lt x y))`;
 
-val empty_def = Define `
+val empty_def = mlDefine `
 empty = Empty`;
 
-val member_def = Define `
+val member_def = mlDefine `
 (member lt x Empty = F) ∧
-(member lt x (Node a y b) =
+(member lt x (Tree a y b) =
   if lt x y then
     member lt x a
   else if lt y x then
@@ -41,52 +35,49 @@ val member_def = Define `
   else
     T)`;
 
-val member_thm = Q.store_thm ("member_thm",
+val insert_def = mlDefine `
+(insert lt x Empty = Tree Empty x Empty) ∧
+(insert lt x (Tree a y b) =
+  if lt x y then
+    Tree (insert lt x a) y b
+  else if lt y x then
+    Tree a y (insert lt x b)
+  else
+    Tree a y b)`;
+
+
+(* Correctness proof *)
+
+val member_correct = Q.store_thm ("member_correct",
 `!lt t x.
-  StrongLinearOrder lt ∧
-  unbalanced_set_ok lt t
+  StrongLinearOrder lt ∧ is_bst lt t
   ⇒
-  (member lt x t = x ∈ unbalanced_set_to_set t)`,
+  (member lt x t = x ∈ tree_to_set t)`,
 induct_on `t` >>
-rw [member_def, unbalanced_set_ok_def, unbalanced_set_to_set_def] >>
+rw [member_def, is_bst_def, tree_to_set_def] >>
 fs [StrongLinearOrder, StrongOrder, irreflexive_def, transitive_def,
     trichotomous] >>
 metis_tac []);
 
-val insert_def = Define `
-(insert lt x Empty = Node Empty x Empty) ∧
-(insert lt x (Node a y b) =
-  if lt x y then
-    Node (insert lt x a) y b
-  else if lt y x then
-    Node a y (insert lt x b)
-  else
-    Node a y b)`;
-
 val insert_set = Q.store_thm ("insert_set",
 `∀lt x t.
-  StrongLinearOrder lt ⇒
-  (unbalanced_set_to_set (insert lt x t) = {x} ∪ unbalanced_set_to_set t)`,
+  StrongLinearOrder lt 
+  ⇒
+  (tree_to_set (insert lt x t) = {x} ∪ tree_to_set t)`,
 induct_on `t` >>
-srw_tac [PRED_SET_AC_ss] [insert_def, unbalanced_set_to_set_def] >>
+srw_tac [PRED_SET_AC_ss] [insert_def, tree_to_set_def] >>
 `x = a` by (fs [StrongLinearOrder, StrongOrder, irreflexive_def,
                 transitive_def, trichotomous] >>
             metis_tac []) >>
 rw []);
 
-val insert_ok = Q.store_thm ("insert_ok",
+val insert_is_bst = Q.store_thm ("insert_is_bst",
 `!lt x t.
-  StrongLinearOrder lt ∧
-  unbalanced_set_ok lt t
+  StrongLinearOrder lt ∧ is_bst lt t
   ⇒
-  unbalanced_set_ok lt (insert lt x t)`,
+  is_bst lt (insert lt x t)`,
 induct_on `t` >>
-rw [unbalanced_set_ok_def, insert_def, unbalanced_set_to_set_def, insert_set] >>
+rw [is_bst_def, insert_def, tree_to_set_def, insert_set] >>
 metis_tac []);
-
-
-val res = translate insert_def;
-val res = translate member_def;
-val res = translate empty_def;
 
 val _ = export_theory ();
